lib: add some heap_path/heap_list lemmas
includes:
- heap_path_prefix
- sym_heap for symmetric heaps
(which replyPrevs_of/replyNexts_of are instances of)
  and related lemmas

Signed-off-by: Miki Tanaka <miki.tanaka@data61.csiro.au>

lib/Heap_List.thy
@@ -8,7 +8,7 @@
    Loosely after ~~/src/HOL/Hoare/Pointer_Examples.thy *)
 
 theory Heap_List
-imports Main
+imports Main "HOL-Library.Prefix_Order"
 begin
 
 (* Given a heap projection that returns the next-pointer for an object at address x,
@@ -78,5 +78,185 @@ lemma heap_list_is_walk':
 lemma heap_list_is_walk:
   "heap_list hp x xs \<Longrightarrow> heap_walk hp x [] = xs"
   using heap_list_is_walk' by fastforce
+
+lemma heap_path_end_unique:
+  "heap_path hp x xs y \<Longrightarrow> heap_path hp x xs y' \<Longrightarrow> y = y'"
+  by (induct xs arbitrary: x; clarsimp)
+
+lemma heap_path_head:
+  "heap_path hp x xs y \<Longrightarrow> xs \<noteq> [] \<Longrightarrow> x = Some (hd xs)"
+  by (induct xs arbitrary: x; clarsimp)
+
+lemma heap_path_non_nil_lookup_next:
+  "heap_path hp x (xs@z#ys) y \<Longrightarrow> hp z = (case ys of [] \<Rightarrow> y | _ \<Rightarrow> Some (hd ys))"
+  by (cases ys; fastforce)
+
+lemma heap_path_prefix:
+  "heap_path hp st ls ed \<Longrightarrow> \<forall>xs\<le>ls. heap_path hp st xs (if xs = [] then st else hp (last xs))"
+  apply clarsimp
+  apply (erule Prefix_Order.prefixE)
+  by (metis append_butlast_last_id heap_path_append heap_path_non_nil_lookup_next list.case(1))
+
+lemma heap_path_butlast:
+  "heap_path hp st ls ed \<Longrightarrow> ls \<noteq> [] \<Longrightarrow> heap_path hp st (butlast ls) (Some (last ls))"
+  by (induct ls rule: rev_induct; simp)
+
+lemma in_list_decompose_takeWhile:
+  "x \<in> set xs \<Longrightarrow>
+   xs = (takeWhile ((\<noteq>) x) xs) @ x # (drop (length (takeWhile ((\<noteq>) x) xs) + 1) xs)"
+  by (induct xs arbitrary: x; clarsimp)
+
+lemma takeWhile_neq_hd_eq_Nil[simp]:
+  "takeWhile ((\<noteq>) (hd xs)) xs = Nil"
+  by (metis (full_types) hd_Cons_tl takeWhile.simps(1) takeWhile.simps(2))
+
+lemma heap_not_in_dom[simp]:
+  "ptr \<notin> dom hp \<Longrightarrow> hp(ptr := None) = hp"
+  by (auto simp: dom_def)
+
+lemma heap_path_takeWhile_lookup_next:
+  "\<lbrakk> heap_path hp st rs ed; r \<in> set rs \<rbrakk>
+   \<Longrightarrow> heap_path hp st (takeWhile ((\<noteq>) r) rs) (Some r)"
+  apply (drule heap_path_prefix)
+  apply (subgoal_tac "takeWhile ((\<noteq>) r) rs @ [r] \<le> rs", fastforce)
+  by (fastforce dest!: in_list_decompose_takeWhile intro: Prefix_Order.prefixI)
+
+lemma heap_path_heap_upd_not_in:
+  "\<lbrakk>heap_path hp st rs ed; r \<notin> set rs\<rbrakk> \<Longrightarrow> heap_path (hp(r:= x)) st rs ed"
+  by (induct rs arbitrary: st; clarsimp)
+
+lemma heap_walk_lb:
+  "heap_walk hp x xs \<ge> xs"
+  apply (induct xs rule: heap_walk.induct; clarsimp)
+  by (metis Prefix_Order.prefixE Prefix_Order.prefixI append_assoc)
+
+lemma heal_walk_Some_nonempty':
+  "heap_walk hp (Some x) [] > []"
+  by (fastforce intro: heap_walk_lb less_le_trans[where y="[x]"])
+
+lemma heal_walk_Some_nonempty:
+  "heap_walk hp (Some x) [] \<noteq> []"
+  by (metis less_list_def heal_walk_Some_nonempty')
+
+lemma heap_walk_Nil_None:
+  "heap_walk hp st [] = [] \<Longrightarrow> st = None"
+   by (case_tac st; simp only: heal_walk_Some_nonempty)
+
+lemma heap_list_last_None:
+  "heap_list hp st xs \<Longrightarrow> xs \<noteq> [] \<Longrightarrow> hp (last xs) = None"
+  by (induct xs rule: rev_induct; clarsimp)
+
+(* sym_heap *)
+
+abbreviation sym_heap where
+  "sym_heap hp hp' \<equiv> \<forall>p p'. hp p = Some p' \<longleftrightarrow> hp' p' = Some p"
+
+lemma sym_heap_symmetric:
+  "sym_heap hp hp' \<longleftrightarrow> sym_heap hp' hp" by blast
+
+lemma sym_heap_None:
+  "\<lbrakk>sym_heap hp hp'; hp p = None\<rbrakk> \<Longrightarrow> \<forall>p'. hp' p' \<noteq> Some p" by force
+
+lemma sym_heap_path_reverse:
+  "sym_heap hp hp' \<Longrightarrow>
+      heap_path hp (Some p) (p#ps) (Some p')
+          \<longleftrightarrow> heap_path hp' (Some p') (p'#(rev ps)) (Some p)"
+  by (induct ps arbitrary: p p' rule: rev_induct; force)
+
+lemma sym_heap_list_rev_Cons:
+  "\<lbrakk>sym_heap hp hp'; heap_list hp (Some p) (p#ps)\<rbrakk>
+  \<Longrightarrow> heap_path hp' (Some (last (p#ps))) (rev ps) (Some p)"
+  supply rev.simps[simp del]
+  apply (induct ps arbitrary: p rule: rev_induct; simp add: rev.simps)
+  by (auto dest!: sym_heap_path_reverse[THEN iffD1])
+
+(* more on heap_path : next/prev in path *)
+
+lemma heap_path_extend:
+  "heap_path hp st (ls @ [p]) (hp p) \<longleftrightarrow> heap_path hp st ls (Some p)"
+  by (induct ls rule: rev_induct; simp)
+
+lemma heap_path_prefix_heap_list:
+  "\<lbrakk>heap_list hp st xs; heap_path hp st ys ed\<rbrakk> \<Longrightarrow> ys \<le> xs"
+  apply (induct xs arbitrary: ys st, simp)
+  apply (case_tac ys; clarsimp)
+  done
+
+lemma distinct_decompose2:
+  "\<lbrakk>distinct xs; xs = ys @ x # y # zs\<rbrakk>
+   \<Longrightarrow> x \<noteq> y \<and> x \<notin> set ys \<and> y \<notin> set ys \<and> x \<notin> set zs \<and> y \<notin> set zs"
+  by (simp add: in_set_conv_decomp)
+
+lemma heap_path_distinct_next_cases: (* the other direction needs sym_heap *)
+  "\<lbrakk>heap_path hp st xs ed; distinct xs; p \<in> set xs; hp p = Some np\<rbrakk>
+  \<Longrightarrow> ed = Some p \<or> ed = Some np \<or> np \<in> set xs"
+  apply (cases ed; simp)
+   apply (frule in_list_decompose_takeWhile)
+   apply (subgoal_tac "heap_list hp st (takeWhile ((\<noteq>) p) xs @ p # drop (length (takeWhile ((\<noteq>) p) xs) + 1) xs)")
+   apply (drule heap_path_non_nil_lookup_next)
+   apply (case_tac "drop (length (takeWhile ((\<noteq>) p) xs) + 1) xs"; simp)
+   apply (metis in_set_dropD list.set_intros(1))
+  apply simp
+  apply (frule in_list_decompose_takeWhile)
+  apply (subgoal_tac "heap_path hp st (takeWhile ((\<noteq>) p) xs @ p # drop (length (takeWhile ((\<noteq>) p) xs) + 1) xs) ed")
+  apply (frule heap_path_non_nil_lookup_next)
+  apply (case_tac "drop (length (takeWhile ((\<noteq>) p) xs) + 1) xs", simp)
+  apply (simp split: if_split_asm)
+  apply (drule (1) distinct_decompose2)
+  apply clarsimp
+  by (metis in_set_dropD list.set_intros(1)) simp
+
+lemma heap_list_next_in_list:
+  "\<lbrakk>heap_list hp st xs; p \<in> set xs; hp p = Some np\<rbrakk>
+  \<Longrightarrow> np \<in> set xs"
+   apply (subgoal_tac "distinct xs")
+   by (fastforce dest!: heap_path_distinct_next_cases) (erule heap_list_distinct)
+
+lemma heap_path_distinct_sym_prev_cases:
+  "\<lbrakk>heap_path hp st xs ed; distinct xs; np \<in> set xs; hp p = Some np; sym_heap hp hp'\<rbrakk>
+  \<Longrightarrow> st = Some np \<or> p \<in> set xs"
+  apply (cases st; simp)
+  apply (rename_tac stp)
+  apply (case_tac "stp = np"; simp)
+  apply (cases xs; simp del: heap_path.simps)
+  apply (frule heap_path_head, simp)
+  apply (cases ed, clarsimp)
+   apply (drule sym_heap_list_rev_Cons, fastforce)
+   apply (drule heap_path_distinct_next_cases[where hp=hp']; simp)
+   apply fastforce
+  apply (simp del: heap_path.simps)
+  apply (drule (1) sym_heap_path_reverse[where hp'=hp', THEN iffD1])
+  apply simp
+  apply (frule heap_path_distinct_next_cases[where hp=hp']; simp)
+  apply fastforce
+  done
+
+lemma heap_list_prev_cases:
+  "\<lbrakk>heap_list hp st xs; np \<in> set xs; hp p = Some np; sym_heap hp hp'\<rbrakk>
+  \<Longrightarrow> st = Some np \<or> p \<in> set xs"
+   apply (subgoal_tac "distinct xs")
+   by (fastforce dest!: heap_path_distinct_sym_prev_cases) (erule heap_list_distinct)
+
+lemma heap_list_prev_not_in:
+  "\<lbrakk>heap_list hp st xs; np \<notin> set xs; hp p = Some np\<rbrakk>
+  \<Longrightarrow> p \<notin> set xs"
+  by (meson heap_list_next_in_list)
+
+lemma heap_path_distinct_prev_not_in:
+  "\<lbrakk>heap_path hp st xs ed; distinct xs; np \<notin> set xs; hp p = Some np; ed \<noteq> Some np; ed \<noteq> Some p\<rbrakk>
+  \<Longrightarrow> p \<notin> set xs"
+  using heap_path_distinct_next_cases
+  by fastforce
+
+lemma heap_path_distinct_next_not_in:
+  "\<lbrakk>heap_path hp st xs ed; distinct xs; p \<notin> set xs; hp p = Some np;
+    sym_heap hp hp'; st \<noteq> Some np\<rbrakk>
+  \<Longrightarrow> np \<notin> set xs"
+  by (fastforce dest!: heap_path_distinct_sym_prev_cases[simplified])
+
+lemma heap_list_next_not_in:
+  "\<lbrakk>heap_list hp st xs; p \<notin> set xs; hp p = Some np; sym_heap hp hp'; st \<noteq> Some np\<rbrakk>
+  \<Longrightarrow> np \<notin> set xs"
+  by (fastforce dest!: heap_list_prev_cases[simplified])
 
 end
